job.v
@@ -14,18 +14,27 @@ Record valid_task (tsk: task) : Prop :=
     job_deadline_positive: job_deadline tsk > 0
   }.
 
-(* A periodic task has an interarrival time *)
-Record periodic_task : Type :=
-  { periodic_task_is_task :> task;
+(* A sporadic task has an interarrival time *)
+Record sporadic_task : Type :=
+  { sporadic_task_is_task :> task;
     task_period : nat
   }.
 
-(* Restrictions on periodic task parameters *)
-Record valid_periodic_task (tsk: periodic_task) : Prop :=
-  { periodic_task_valid: valid_task tsk;
+(* Restrictions on sporadic task parameters *)
+Record valid_sporadic_task (tsk: sporadic_task) : Prop :=
+  { sporadic_task_valid: valid_task tsk;
     job_interarrival:
-        forall t1 t2, t1 <> t2
+        forall t1 t2, (t1 <> t2
                       /\ job_arrival tsk t1
-                      /\ job_arrival tsk t2
+                      /\ job_arrival tsk t2)
                       -> t1 <= t2 + task_period tsk
   }.
+
+Definition job_interarrival_fixed (tsk: sporadic_task) := forall t1 t2,
+                      (t1 <> t2
+                      /\ job_arrival tsk t1
+                      /\ job_arrival tsk t2)
+                      -> t1 <= t2 + task_period tsk.
+
+Definition periodic_task := {tsk: sporadic_task | valid_sporadic_task tsk
+                                                  /\ job_interarrival_fixed tsk }.
